@prefix : <http://iot.linkeddata.es/def/wot#> .
@prefix dc: <http://purl.org/dc/elements/1.1/> .
@prefix vs: <http://www.w3.org/2003/06/sw-vocab-status/ns#> .
@prefix geo: <http://www.w3.org/2003/01/geo/wgs84_pos#> .
@prefix owl: <http://www.w3.org/2002/07/owl#> .
@prefix rdf: <http://www.w3.org/1999/02/22-rdf-syntax-ns#> .
@prefix wot: <http://xmlns.com/wot/0.1/> .
@prefix xml: <http://www.w3.org/XML/1998/namespace> .
@prefix xsd: <http://www.w3.org/2001/XMLSchema#> .
@prefix doap: <http://usefulinc.com/ns/doap#> .
@prefix foaf: <http://xmlns.com/foaf/0.1/> .
@prefix prov: <http://www.w3.org/ns/prov#> .
@prefix rdfs: <http://www.w3.org/2000/01/rdf-schema#> .
@prefix vann: <http://purl.org/vocab/vann/> .
@prefix saref: <https://w3id.org/saref#> .
@prefix dcterms: <http://purl.org/dc/terms/> .
@base <http://iot.linkeddata.es/def/wot#> .

<http://iot.linkeddata.es/def/wot#> rdf:type owl:Ontology ;
                                     dcterms:creator <http://purl.org/net/mpoveda> ;
                                     owl:versionInfo "0.0.4" ;
                                     dcterms:creator <http://www.garcia-castro.com/foaf.rdf#me> ;
                                     vann:preferredNamespacePrefix "wot" ;
                                     dcterms:license <http://purl.org/NET/rdflicense/cc-by4.0> ;
                                     vann:preferredNamespaceUri "http://iot.linkeddata.es/def/wot" ;
                                     rdfs:comment "This ontology aims to model the Web of Things domain according to the w3c Interest Group (http://w3c.github.io/wot/)"@en ;
                                     dc:title "Ontology model for Web of Things"@en ;
                                     dcterms:creator <http://www.oeg-upm.net/index.php/en/universitystaff/402-fserena/> ;
                                     dc:publisher <http://www.oeg-upm.net/> .

#################################################################
#    Annotation properties
#################################################################

###  http://www.w3.org/2003/06/sw-vocab-status/ns#term_status
vs:term_status rdf:type owl:AnnotationProperty .


#################################################################
#    Object Properties
#################################################################

###  http://iot.linkeddata.es/def/wot#contains
:contains rdf:type owl:ObjectProperty ;
          rdfs:comment "A property between a thing and its components. For example, virtual things can contain virtual things whiel physical things can contain physicial things."@en ;
          rdfs:label "contains"@en ;
          rdfs:seeAlso "ISO/IEC CC 30141. Information technology - Internet of Things Reference architecutre (ioT RA)" .


###  http://iot.linkeddata.es/def/wot#describes
:describes rdf:type owl:ObjectProperty ;
           owl:inverseOf :isDescribedBy ;
           rdfs:comment "Link from a thing description to the thing being described"@en ;
           rdfs:label "describes thing"@en ;
           owl:deprecated "true"^^xsd:boolean .


###  http://iot.linkeddata.es/def/wot#hasInputData
:hasInputData rdf:type owl:ObjectProperty ;
              rdfs:comment "link to the n-ary class that allows the declaration of the data type and unit of measure expected by an interaction pattern."@en ;
              rdfs:label "has input data"@en .


###  http://iot.linkeddata.es/def/wot#hasMediaType
:hasMediaType rdf:type owl:ObjectProperty ;
              rdfs:comment "link to the media types sopported by an endpoint"@en ;
              rdfs:label "has media type"@en .


###  http://iot.linkeddata.es/def/wot#hasOutputData
:hasOutputData rdf:type owl:ObjectProperty ;
               rdfs:comment "link to the n-ary class that allows the declaration of the data type and unit of measure provided by an interaction pattern."@en ;
               rdfs:label "has output data"@en .


###  http://iot.linkeddata.es/def/wot#hasValueType
:hasValueType rdf:type owl:ObjectProperty ;
              rdfs:comment "Link to the data type used for the values provided following a given data format"@en ;
              rdfs:label "has value type"@en .


###  http://iot.linkeddata.es/def/wot#isAccessibleThrough
:isAccessibleThrough rdf:type owl:ObjectProperty ;
                     rdfs:comment "Indicates the endpoints from which an interaction pattern is accessible"@en ;
                     rdfs:label "is accessible through"@en .


###  http://iot.linkeddata.es/def/wot#isDescribedBy
:isDescribedBy rdf:type owl:ObjectProperty ;
               rdfs:comment "Relation from a thing to its thing descriptions"@en ;
               rdfs:label "is described by"@en ;
               owl:deprecated "true"^^xsd:boolean .


###  http://iot.linkeddata.es/def/wot#isMeasuredIn
:isMeasuredIn rdf:type owl:ObjectProperty ;
              rdfs:comment "A relation between a measurement and the unit of measure in which the measurement value is expressed."@en ;
              rdfs:label "is measured in"@en .


###  http://iot.linkeddata.es/def/wot#isProvidedOverProtocol
:isProvidedOverProtocol rdf:type owl:ObjectProperty ,
                                 owl:FunctionalProperty ;
                        rdfs:comment "Relates an endpoint with the communication protocol it is served over. A given endpoint can be provided over at most one protocol."@en ;
                        rdfs:label "is provided over protocol"@en .


###  http://iot.linkeddata.es/def/wot#isRelativeTo
:isRelativeTo rdf:type owl:ObjectProperty ;
              rdfs:comment "Link from a relative endpoint to the (non relative) endpoint to which it is relative."@en ;
              rdfs:label "is relative to"@en .


###  http://iot.linkeddata.es/def/wot#providedBy
:providedBy rdf:type owl:ObjectProperty ;
            rdfs:label "providedBy"@en ;
            vs:term_status "propose for deletion" .


###  http://iot.linkeddata.es/def/wot#providesInteractionPattern
:providesInteractionPattern rdf:type owl:ObjectProperty ;
                            rdfs:domain :InteractionPattern ;
                            rdfs:comment "Link from a thing to the interaction patterns it provides"@en ;
                            rdfs:label "provides interaction pattern"@en .


#################################################################
#    Data properties
#################################################################

###  http://iot.linkeddata.es/def/wot#baseURI
:baseURI rdf:type owl:DatatypeProperty ;
         rdfs:domain :Thing ;
         rdfs:range xsd:string ;
         rdfs:comment "Define base URI that is valid for all defined local interaction resources. All other URIs in the TD must then be resolved using the algorithm defined in [RFC3986]. This field is optional. (Definition taken from http://w3c.github.io/wot/current-practices/wot-practices#thing-metadata)"@en ;
         rdfs:label "base URI"@en .


###  http://iot.linkeddata.es/def/wot#defaultValue
:defaultValue rdf:type owl:DatatypeProperty ;
              rdfs:range rdfs:Literal ;
              rdfs:label "defaultValue"@en ;
              vs:term_status "unstable. where does this req come from?"@en .


###  http://iot.linkeddata.es/def/wot#href
:href rdf:type owl:DatatypeProperty ,
               owl:FunctionalProperty ;
      rdfs:range xsd:string ;
      rdfs:comment "URI of the endpoint where an interaction pattern is provided"@en ;
      rdfs:label "href"@en .


###  http://iot.linkeddata.es/def/wot#interactionName
:interactionName rdf:type owl:DatatypeProperty ;
                 rdfs:subPropertyOf :name ;
                 rdfs:comment "Name of an interaction pattern" ;
                 rdfs:label "interaction name"@en .


###  http://iot.linkeddata.es/def/wot#isRequired
:isRequired rdf:type owl:DatatypeProperty ,
                     owl:FunctionalProperty ;
            rdfs:range xsd:boolean ;
            rdfs:comment "Boolean value that indicates whether a property is required to be present."@en ;
            rdfs:label "is required"@en .


###  http://iot.linkeddata.es/def/wot#isWritable
:isWritable rdf:type owl:DatatypeProperty ,
                     owl:FunctionalProperty ;
            rdfs:range xsd:boolean ;
            rdfs:comment "Boolean value that indicates whether a property is writable"@en ;
            rdfs:label "is writable"@en .


###  http://iot.linkeddata.es/def/wot#name
:name rdf:type owl:DatatypeProperty ;
      rdfs:range xsd:string ;
      rdfs:comment "General attribute for names assigned to any type of concept" ;
      rdfs:label "name"@en .


###  http://iot.linkeddata.es/def/wot#thingName
:thingName rdf:type owl:DatatypeProperty ;
           rdfs:subPropertyOf :name ;
           rdfs:comment "Name of a thing, physical or virtual" ;
           rdfs:label "thing name"@en .


#################################################################
#    Classes
#################################################################

###  http://iot.linkeddata.es/def/wot#Action
:Action rdf:type owl:Class ;
        rdfs:subClassOf :InteractionPattern ,
                        [ rdf:type owl:Restriction ;
                          owl:onProperty :hasInputData ;
                          owl:allValuesFrom :DataFormat
                        ] ,
                        [ rdf:type owl:Restriction ;
                          owl:onProperty :hasOutputData ;
                          owl:allValuesFrom :DataFormat
                        ] ;
        rdfs:comment "The Action interaction pattern targets changes or processes on a Thing that take a certain time to complete (i.e., actions cannot be applied instantaneously like property writes). Examples include an LED fade in, moving a robot, brewing a cup of coffee, etc. Usually, ongoing Actions are modelled as Task resources, which are created when an Action invocation is received by the Thing. (Definition taken from http://w3c.github.io/wot/current-practices/wot-practices#action)"@en ;
        rdfs:label "Action"@en .


###  http://iot.linkeddata.es/def/wot#CommunicationProtocol
:CommunicationProtocol rdf:type owl:Class ;
                       owl:disjointWith :Property ,
                                        :WoTInterface ,
                                        saref:Service ;
                       rdfs:comment "A protocol is an agreement between the communicating parties on how communication is to proceed. (Definition taken from \"Tanenbaum, A. S. (2003). Computer networks, 4-th edition. ed: Prentice Hall.\")"@en ;
                       rdfs:label "Communication protocol"@en .


###  http://iot.linkeddata.es/def/wot#DataFormat
:DataFormat rdf:type owl:Class ;
            rdfs:subClassOf [ rdf:type owl:Restriction ;
                              owl:onProperty :hasValueType ;
                              owl:allValuesFrom :DataType
                            ] ,
                            [ rdf:type owl:Restriction ;
                              owl:onProperty :isMeasuredIn ;
                              owl:allValuesFrom :UnitOfMeasure
                            ] ;
            rdfs:comment "N-ary class defined to allow the representation of pairs (data type, unit of measure) that are expected as input data or output data of a given interaction pattern."@en ;
            rdfs:label "Data format"@en .


###  http://iot.linkeddata.es/def/wot#DataType
:DataType rdf:type owl:Class ;
          rdfs:comment "Set of distinct values, characterized by properties of those values, and by operations on those values (definition taken from ISO/IEC 11404:2007)"@en ;
          rdfs:label "Data type"@en ;
          rdfs:seeAlso "https://www.iso.org/obp/ui/#iso:std:iso-iec:11404:ed-2:v1:en"@en .


###  http://iot.linkeddata.es/def/wot#Endpoint
:Endpoint rdf:type owl:Class ;
          rdfs:subClassOf [ rdf:type owl:Restriction ;
                            owl:onProperty :isProvidedOverProtocol ;
                            owl:someValuesFrom :CommunicationProtocol
                          ] ,
                          [ rdf:type owl:Restriction ;
                            owl:onProperty :hasMediaType ;
                            owl:allValuesFrom :MediaType
                          ] ,
                          [ rdf:type owl:Restriction ;
                            owl:onProperty :href ;
                            owl:someValuesFrom xsd:string
                          ] ;
          rdfs:comment "A URL where a service can be accessed by a client application. A service might have more than one endpoint."@en ;
          rdfs:label "Endpoint"@en .


###  http://iot.linkeddata.es/def/wot#Event
:Event rdf:type owl:Class ;
       rdfs:subClassOf :InteractionPattern ,
                       [ rdf:type owl:Restriction ;
                         owl:onProperty :hasOutputData ;
                         owl:allValuesFrom :DataFormat
                       ] ;
       rdfs:comment "The Event interaction pattern enables a mechanism to be notified by a Thing on a certain condition. (Description taken from http://w3c.github.io/wot/current-practices/wot-practices#event)"@en ;
       rdfs:label "Event"@en .


###  http://iot.linkeddata.es/def/wot#InteractionPattern
:InteractionPattern rdf:type owl:Class ;
                    rdfs:subClassOf [ rdf:type owl:Restriction ;
                                      owl:onProperty :isAccessibleThrough ;
                                      owl:someValuesFrom :Endpoint
                                    ] ,
                                    [ rdf:type owl:Restriction ;
                                      owl:onProperty :providedBy ;
                                      owl:someValuesFrom :WebResource
                                    ] ,
                                    [ rdf:type owl:Restriction ;
                                      owl:onProperty :interactionName ;
                                      owl:someValuesFrom xsd:string
                                    ] ;
                    rdfs:comment "An interaction in the context of the Web of Things is an exchange of data between a Web client and a Thing. This data can be either given as input by the client, returned as output by the Thing or both. Three interaction patterns have been defined so far: Property, Action and Event. (Definition taken from http://w3c.github.io/wot/current-practices/wot-practices#interaction-patterns)"@en ;
                    rdfs:label "Interaction pattern"@en .


###  http://iot.linkeddata.es/def/wot#MediaType
:MediaType rdf:type owl:Class ;
           rdfs:comment """Represent the label (estructured into trees) used to identify the content type os a particular protocols, including but not limited to HTTP [RFC2616] and MIME [RFC2045], which are capable of carrying arbitrary labeled content. (Definicion adapted from https://tools.ietf.org/html/rfc6838).

The location of the media type registry is http://www.iana.org/assignments/media-types/"""@en ;
           rdfs:label "MediaType"@en .


###  http://iot.linkeddata.es/def/wot#PhysicalThing
:PhysicalThing rdf:type owl:Class ;
               rdfs:subClassOf :Thing ,
                               [ rdf:type owl:Restriction ;
                                 owl:onProperty :contains ;
                                 owl:allValuesFrom :PhysicalThing
                               ] ;
               rdfs:comment """A physical entity is a real-world thing. A physical entity is a specialization of entity. A physical entity may contain other physical entities. A physical entity is a discrete, identifiable part of the physical environment that is of interest to the user for the completion of her goal. Physical entities can be almost any physical object or environment; from humans or animals to cars; from store or logistics chain items to computers; from electronic appliances to closed or open environments.

(Definition taken from 
ISO/IEC CC 30141. Information technology - Internet of Things Reference architecutre (IoT RA))"""@en ,
                            "Any entity that has a proper space region."@en ;
               rdfs:label "Physical thing"@en ;
               rdfs:seeAlso "ISO/IEC CC 30141. Information technology - Internet of Things Reference architecutre (IoT RA)"@en .


###  http://iot.linkeddata.es/def/wot#Property
:Property rdf:type owl:Class ;
          rdfs:subClassOf :InteractionPattern ,
                          [ rdf:type owl:Restriction ;
                            owl:onProperty :hasOutputData ;
                            owl:someValuesFrom :DataFormat
                          ] ,
                          [ rdf:type owl:Restriction ;
                            owl:onProperty :hasOutputData ;
                            owl:allValuesFrom :DataFormat
                          ] ,
                          [ rdf:type owl:Restriction ;
                            owl:onProperty :isRequired ;
                            owl:allValuesFrom xsd:boolean
                          ] ,
                          [ rdf:type owl:Restriction ;
                            owl:onProperty :isWritable ;
                            owl:allValuesFrom xsd:boolean
                          ] ;
          owl:disjointWith :WoTInterface ,
                           saref:Service ;
          rdfs:comment "Property provides readable and/or writeable data that can be static (e.g., supported mode, rated output voltage, etc.) or dynamic (e.g., current fill level of water, minimum recorded temperature, etc.).  (Definition taken from http://w3c.github.io/wot/current-practices/wot-practices#property)"@en ;
          rdfs:label "Property"@en .


###  http://iot.linkeddata.es/def/wot#RelativeEndpoint
:RelativeEndpoint rdf:type owl:Class ;
                  rdfs:subClassOf :Endpoint ,
                                  [ rdf:type owl:Restriction ;
                                    owl:onProperty :isRelativeTo ;
                                    owl:maxQualifiedCardinality "1"^^xsd:nonNegativeInteger ;
                                    owl:onClass [ owl:intersectionOf ( :Endpoint
                                                                       [ rdf:type owl:Class ;
                                                                         owl:complementOf :RelativeEndpoint
                                                                       ]
                                                                     ) ;
                                                  rdf:type owl:Class
                                                ]
                                  ] ;
                  rdfs:comment "An endpoint which is relative (its href is composed by a relative path and an absolute one given by another endpoint) to an endpoint which can not be relative."@en ;
                  rdfs:label "Relative endpoint"@en .


###  http://iot.linkeddata.es/def/wot#Thing
:Thing rdf:type owl:Class ;
       rdfs:subClassOf [ rdf:type owl:Restriction ;
                         owl:onProperty :isAccessibleThrough ;
                         owl:allValuesFrom :Endpoint
                       ] ,
                       [ rdf:type owl:Restriction ;
                         owl:onProperty :isDescribedBy ;
                         owl:allValuesFrom :ThingDescription
                       ] ,
                       [ rdf:type owl:Restriction ;
                         owl:onProperty :providesInteractionPattern ;
                         owl:allValuesFrom :InteractionPattern
                       ] ;
       rdfs:comment """An thing is anything (both physical and non-physical) which has a distinct and independent existence. Every thing has a unique identity. (Definition adapted from 
ISO/IEC CC 30141. Information technology - Internet of Things Reference architecutre (IoT RA))"""@en ,
                    "The abstract concept of a physical entity that can either be a real-world artifact, such as a device, or a virtual entity that represents physicality, such as a room or group of devices"@en ;
       rdfs:label "Thing"@en .


###  http://iot.linkeddata.es/def/wot#ThingDescription
:ThingDescription rdf:type owl:Class ;
                  rdfs:subClassOf [ rdf:type owl:Restriction ;
                                    owl:onProperty :describes ;
                                    owl:someValuesFrom :Thing
                                  ] ,
                                  [ rdf:type owl:Restriction ;
                                    owl:onProperty :describes ;
                                    owl:allValuesFrom :Thing
                                  ] ;
                  rdfs:comment "A digital representation encapsulates a physical object accessible via Web services"@en ;
                  rdfs:label "Thing description"@en ;
                  owl:deprecated "true"^^xsd:boolean .


###  http://iot.linkeddata.es/def/wot#UnitOfMeasure
:UnitOfMeasure rdf:type owl:Class ;
               rdfs:comment "The unit of measure is a standard for measurement of a quantity, such as a Property. For example, Temperature is a property and centigrade (or Celsius) is a unit of temperature that represents a definite predetermined temperature: when we say 20 centigrade, we actually mean 20 times the definite predetermined temperature unit called \"centigrade\". Our definition is based on the definition of unit of measure in the Ontology of units of Measure (OM). (Definition adapted from SAREF ontology)"@en ;
               rdfs:label "Unit of measure"@en .


###  http://iot.linkeddata.es/def/wot#VirtualThing
:VirtualThing rdf:type owl:Class ;
              rdfs:subClassOf :Thing ,
                              [ rdf:type owl:Restriction ;
                                owl:onProperty :contains ;
                                owl:allValuesFrom :VirtualThing
                              ] ;
              rdfs:comment """A virtual entity is a digital representation of a physical entity, contained within a service. A virtual entity interacts through an endpoint. A virtual entity represents a physical entity.

(Definition taken from 
ISO/IEC CC 30141. Information technology - Internet of Things Reference architecutre (IoT RA))"""@en ;
              rdfs:label "Virtual thing"@en ;
              rdfs:seeAlso "ISO/IEC CC 30141. Information technology - Internet of Things Reference architecutre (ioT RA)"@en .


###  http://iot.linkeddata.es/def/wot#WebResource
:WebResource rdf:type owl:Class ;
             rdfs:label "WebResource"@en ;
             vs:term_status "unstable" .


###  http://iot.linkeddata.es/def/wot#WoTInterface
:WoTInterface rdf:type owl:Class ;
              rdfs:subClassOf [ rdf:type owl:Restriction ;
                                owl:onProperty :providesInteractionPattern ;
                                owl:allValuesFrom :InteractionPattern
                              ] ;
              rdfs:comment "A WoT interface is also a web API that follows the recommendations of the WoT Interest Group."@en ,
                           "Resource-oriented Web interface (often called \"Web API\") that allows access to servients over the network using different Protocol Bindings."@en ;
              rdfs:label "Web of Thing interface"@en ;
              vs:term_status "proposed for deletion" .


###  https://w3id.org/saref#Service
saref:Service rdf:type owl:Class ;
              rdfs:comment "A service is a representation of a function to a network that makes the function discoverable, registerable, remotely controllable by other devices in the network. A service can represent one or more functions. A Service is offered by a device that wants (a certain set of) its function(s) to be discoverable, registerable, remotely controllable by other devices in the network. A Service must specify the device that is offering the service, the function(s) to be represented, and the (input and output) parameters necessary to operate the service."@en ;
              rdfs:isDefinedBy saref: ;
              rdfs:label "Service"@en ;
              vs:term_status "unstable" .


###  Generated by the OWL API (version 4.2.6.20160910-2108) https://github.com/owlcs/owlapi
